shorten names

src/phase2/freedom_of_action/non_flexible_case.lean
@@ -15,7 +15,7 @@ open quiver set sum with_bot
 universe u
 
 namespace con_nf
-namespace allowable_partial_perm
+namespace allowable_spec
 
 variables [params.{u}]
 
@@ -24,7 +24,7 @@ open struct_perm spec
 variables {α : Λ} [phase_2_core_assumptions α] [phase_2_positioned_assumptions α]
   [typed_positions.{}] [phase_2_assumptions α] {B : le_index α}
 
-variables {B} {σ : allowable_partial_perm B} ⦃β : Λ⦄ ⦃γ : type_index⦄ ⦃δ : Λ⦄
+variables {B} {σ : allowable_spec B} ⦃β : Λ⦄ ⦃γ : type_index⦄ ⦃δ : Λ⦄
 
 /-- Since the designated support of `t` is included in `σ`, any allowable permutation `π'` that
 satisfies `σ` at the lower level gives the same result for the image of `f_map_path hγ hδ t`.
@@ -33,7 +33,7 @@ chosen any other permutation and arrived at the same value for the image of `f_m
 
 Don't prove this unless we need it - it sounds like an important mathematical point but potentially
 not for the formalisation itself. -/
-lemma non_flexible_union_unique (hγ : γ < β) (hδ : δ < β) (hγδ : γ ≠ δ)
+lemma non_flex_union_unique (hγ : γ < β) (hδ : δ < β) (hγδ : γ ≠ δ)
   (C : path (B : type_index) β)
   (t : tangle_path ((lt_index.mk' hγ (B.path.comp C)) : le_index α))
   (π : allowable_path (lt_index.mk' (coe_lt_coe.mpr hδ) (B.path.comp C) : le_index α))
@@ -45,7 +45,7 @@ lemma non_flexible_union_unique (hγ : γ < β) (hδ : δ < β) (hγδ : γ ≠ 
         π.to_struct_perm • (f_map_path hγ hδ t).to_near_litter :=
 sorry
 
-private noncomputable def new_non_flexible_constraint (hγ : γ < β) (hδ : δ < β) (hγδ : γ ≠ δ)
+private noncomputable def new_non_flex_constraint (hγ : γ < β) (hδ : δ < β) (hγδ : γ ≠ δ)
   {C : path (B : type_index) β}
   (t : tangle_path ((lt_index.mk' hγ (B.path.comp C)) : le_index α))
   {π : allowable_path (lt_index.mk' (coe_lt_coe.mpr hδ) (B.path.comp C) : le_index α)}
@@ -61,42 +61,42 @@ variables (hγ : γ < β) (hδ : δ < β) (hγδ : γ ≠ δ) {C : path (B : typ
   {π : allowable_path (lt_index.mk' (coe_lt_coe.mpr hδ) (B.path.comp C) : le_index α)}
   (hπ : π.to_struct_perm.satisfies $ σ.val.lower (C.cons $ coe_lt_coe.mpr hδ))
 
-@[simp] lemma mem_new_non_flexible_constraint (c : binary_condition B) :
-  c ∈ ({new_non_flexible_constraint hγ hδ hγδ t hπ} : spec B) ↔
+@[simp] lemma mem_new_non_flex_constraint (c : binary_condition B) :
+  c ∈ ({new_non_flex_constraint hγ hδ hγδ t hπ} : spec B) ↔
   c = (inr ((f_map_path hγ hδ t).to_near_litter,
       struct_perm.derivative (path.nil.cons $ bot_lt_coe _)
         π.to_struct_perm • (f_map_path hγ hδ t).to_near_litter),
       (C.cons $ coe_lt_coe.mpr hδ).cons (bot_lt_coe _)) :=
 by rw spec.mem_singleton; refl
 
-@[simp] lemma inl_eq_new_non_flexible_constraint (a : atom × atom) (A : extended_index B) :
-  ((inl a, A) : binary_condition B) = new_non_flexible_constraint hγ hδ hγδ t hπ ↔ false :=
-by unfold new_non_flexible_constraint; simp only [prod.mk.inj_iff, false_and]
+@[simp] lemma inl_eq_new_non_flex_constraint (a : atom × atom) (A : extended_index B) :
+  ((inl a, A) : binary_condition B) = new_non_flex_constraint hγ hδ hγδ t hπ ↔ false :=
+by unfold new_non_flex_constraint; simp only [prod.mk.inj_iff, false_and]
 
-@[simp] lemma inr_eq_new_non_flexible_constraint
+@[simp] lemma inr_eq_new_non_flex_constraint
   (N : near_litter × near_litter) (A : extended_index B) :
-  ((inr N, A) : binary_condition B) = new_non_flexible_constraint hγ hδ hγδ t hπ ↔
+  ((inr N, A) : binary_condition B) = new_non_flex_constraint hγ hδ hγδ t hπ ↔
   N = ((f_map_path hγ hδ t).to_near_litter,
       struct_perm.derivative (path.nil.cons $ bot_lt_coe _)
         π.to_struct_perm • (f_map_path hγ hδ t).to_near_litter) ∧
   A = (C.cons $ coe_lt_coe.mpr hδ).cons (bot_lt_coe _) :=
-by unfold new_non_flexible_constraint; simp only [prod.mk.inj_iff]
+by unfold new_non_flex_constraint; simp only [prod.mk.inj_iff]
 
-lemma non_flexible_union_one_to_one_forward :
-  spec.one_to_one_forward (σ.val ⊔ {new_non_flexible_constraint hγ hδ hγδ t hπ}) :=
+lemma non_flex_union_one_to_one_forward :
+  spec.one_to_one_forward (σ.val ⊔ {new_non_flex_constraint hγ hδ hγδ t hπ}) :=
 begin
   intro A, split,
   { rintros b c (hc | hc) d (hd | hd),
     { exact (σ.property.forward.one_to_one A).atom b hc hd, },
-    { simpa only [coe_singleton, mem_singleton_iff, inl_eq_new_non_flexible_constraint]
+    { simpa only [coe_singleton, mem_singleton_iff, inl_eq_new_non_flex_constraint]
         using hd, },
-    { simpa only [coe_singleton, mem_singleton_iff, inl_eq_new_non_flexible_constraint]
+    { simpa only [coe_singleton, mem_singleton_iff, inl_eq_new_non_flex_constraint]
         using hc, },
-    { simpa only [coe_singleton, mem_singleton_iff, inl_eq_new_non_flexible_constraint]
+    { simpa only [coe_singleton, mem_singleton_iff, inl_eq_new_non_flex_constraint]
         using hc, }, },
   { rintros N M₁ (hM₁ | hM₁) M₂ (hM₂ | hM₂),
     { exact (σ.property.forward.one_to_one A).near_litter N hM₁ hM₂, },
-    { simp only [coe_singleton, mem_singleton_iff, inr_eq_new_non_flexible_constraint,
+    { simp only [coe_singleton, mem_singleton_iff, inr_eq_new_non_flex_constraint,
         prod.mk.inj_iff] at hM₂,
       transitivity struct_perm.derivative (path.nil.cons $ bot_lt_coe _) π⁻¹.to_struct_perm • N,
       { cases hM₂.2,
@@ -109,7 +109,7 @@ begin
           simp only [map_inv, inv_mul_self, one_smul], },
         { exact hM₁, } },
       { rw [map_inv, map_inv, inv_smul_eq_iff, hM₂.1.1, hM₂.1.2], } },
-    { simp only [coe_singleton, mem_singleton_iff, inr_eq_new_non_flexible_constraint,
+    { simp only [coe_singleton, mem_singleton_iff, inr_eq_new_non_flex_constraint,
         prod.mk.inj_iff] at hM₁,
       transitivity struct_perm.derivative (path.nil.cons $ bot_lt_coe _) π⁻¹.to_struct_perm • N,
       { rw [map_inv, map_inv, eq_inv_smul_iff, hM₁.1.1, hM₁.1.2], },
@@ -122,31 +122,31 @@ begin
           rw ← mul_smul,
           simp only [map_inv, inv_mul_self, one_smul], },
         { exact hM₂, } } },
-    { simp only [coe_singleton, mem_singleton_iff, inr_eq_new_non_flexible_constraint,
+    { simp only [coe_singleton, mem_singleton_iff, inr_eq_new_non_flex_constraint,
         prod.mk.inj_iff] at hM₁ hM₂,
       rw hM₁.1.1, rw hM₂.1.1, } },
 end
 
-lemma non_flexible_union_one_to_one_backward :
-  spec.one_to_one_forward (σ.val ⊔ {new_non_flexible_constraint hγ hδ hγδ t hπ})⁻¹ :=
+lemma non_flex_union_one_to_one_backward :
+  spec.one_to_one_forward (σ.val ⊔ {new_non_flex_constraint hγ hδ hγδ t hπ})⁻¹ :=
 begin
   rw sup_inv,
   intro A, split,
   { rintros b c (hc | hc) d (hd | hd),
     { exact (σ.property.backward.one_to_one A).atom b hc hd, },
     { simpa only [coe_inv, coe_singleton, inv_singleton, binary_condition.inv_def,
-        mem_singleton_iff, prod.mk.inj_iff, new_non_flexible_constraint, sum.map_inr,
+        mem_singleton_iff, prod.mk.inj_iff, new_non_flex_constraint, sum.map_inr,
         false_and] using hd, },
     { simpa only [coe_inv, coe_singleton, inv_singleton, binary_condition.inv_def,
-        mem_singleton_iff, prod.mk.inj_iff, new_non_flexible_constraint, sum.map_inr,
+        mem_singleton_iff, prod.mk.inj_iff, new_non_flex_constraint, sum.map_inr,
         false_and] using hc, },
     { simpa only [coe_inv, coe_singleton, inv_singleton, binary_condition.inv_def,
-        mem_singleton_iff, prod.mk.inj_iff, new_non_flexible_constraint, sum.map_inr,
+        mem_singleton_iff, prod.mk.inj_iff, new_non_flex_constraint, sum.map_inr,
         false_and] using hc, }, },
   { rintros N M₁ (hM₁ | hM₁) M₂ (hM₂ | hM₂),
     { exact (σ.property.backward.one_to_one A).near_litter N hM₁ hM₂, },
     { simp only [coe_inv, coe_singleton, set.mem_inv, mem_singleton_iff, binary_condition.inv_def,
-        sum.map_inr, prod.swap, new_non_flexible_constraint, prod.mk.inj_iff] at hM₂,
+        sum.map_inr, prod.swap, new_non_flex_constraint, prod.mk.inj_iff] at hM₂,
       transitivity struct_perm.derivative (path.nil.cons $ bot_lt_coe _) π.to_struct_perm • N,
       { cases hM₂.2,
         have := hπ (_ : (inr (N, M₁),
@@ -157,7 +157,7 @@ begin
         { exact hM₁, } },
       { rw [hM₂.1.1, hM₂.1.2], } },
     { simp only [coe_inv, coe_singleton, set.mem_inv, mem_singleton_iff, binary_condition.inv_def,
-        sum.map_inr, prod.swap, new_non_flexible_constraint, prod.mk.inj_iff] at hM₁,
+        sum.map_inr, prod.swap, new_non_flex_constraint, prod.mk.inj_iff] at hM₁,
       transitivity struct_perm.derivative (path.nil.cons $ bot_lt_coe _) π.to_struct_perm • N,
       { rw [hM₁.1.1, hM₁.1.2], },
       { cases hM₁.2,
@@ -168,32 +168,32 @@ begin
         { dsimp only [satisfies_cond, sum.elim_inr] at this, rw ← this, },
         { exact hM₂, } }, },
     { simp only [coe_inv, coe_singleton, inv_singleton, binary_condition.inv_def,
-        mem_singleton_iff, prod.mk.inj_iff, new_non_flexible_constraint, map_inr, prod.swap]
+        mem_singleton_iff, prod.mk.inj_iff, new_non_flex_constraint, map_inr, prod.swap]
         at hM₁ hM₂,
       rw hM₁.1.1, rw hM₂.1.1, } },
 end
 
-lemma non_flexible_union_atom_cond_forward :
-  ∀ L C, spec.atom_cond (σ.val ⊔ {new_non_flexible_constraint hγ hδ hγδ t hπ}) L C :=
+lemma non_flex_union_atom_cond_forward :
+  ∀ L C, spec.atom_cond (σ.val ⊔ {new_non_flex_constraint hγ hδ hγδ t hπ}) L C :=
 sorry
 
-lemma non_flexible_union_atom_cond_backward :
-  ∀ L C, spec.atom_cond (σ.val ⊔ {new_non_flexible_constraint hγ hδ hγδ t hπ})⁻¹ L C :=
+lemma non_flex_union_atom_cond_backward :
+  ∀ L C, spec.atom_cond (σ.val ⊔ {new_non_flex_constraint hγ hδ hγδ t hπ})⁻¹ L C :=
 sorry
 
-lemma non_flexible_union_near_litter_cond_forward :
-  ∀ N₁ N₂ C, spec.near_litter_cond (σ.val ⊔ {new_non_flexible_constraint hγ hδ hγδ t hπ}) N₁ N₂ C :=
+lemma non_flex_union_near_litter_cond_forward :
+  ∀ N₁ N₂ C, spec.near_litter_cond (σ.val ⊔ {new_non_flex_constraint hγ hδ hγδ t hπ}) N₁ N₂ C :=
 sorry
 
-lemma non_flexible_union_near_litter_cond_backward :
+lemma non_flex_union_near_litter_cond_backward :
   ∀ N₁ N₂ C,
-    spec.near_litter_cond (σ.val ⊔ {new_non_flexible_constraint hγ hδ hγδ t hπ})⁻¹ N₁ N₂ C :=
+    spec.near_litter_cond (σ.val ⊔ {new_non_flex_constraint hγ hδ hγδ t hπ})⁻¹ N₁ N₂ C :=
 sorry
 
-lemma non_flexible_union_non_flexible_cond_forward :
-  spec.non_flexible_cond B (σ.val ⊔ {new_non_flexible_constraint hγ hδ hγδ t hπ}) :=
+lemma non_flex_union_non_flex_cond_forward :
+  spec.non_flex_cond B (σ.val ⊔ {new_non_flex_constraint hγ hδ hγδ t hπ}) :=
 begin
-  unfold spec.non_flexible_cond,
+  unfold spec.non_flex_cond,
   intros β γ δ hγ hδ hγδ N C t hf π hπ,
   unfold struct_perm.satisfies struct_perm.satisfies_cond at hπ,
   have h := hπ hf,
@@ -209,12 +209,12 @@ begin
     allowable_path.smul_derivative_bot],
 end
 
-lemma non_flexible_union_non_flexible_cond_backward :
-  spec.non_flexible_cond B (σ.val ⊔ {new_non_flexible_constraint hγ hδ hγδ t hπ})⁻¹ :=
+lemma non_flex_union_non_flex_cond_backward :
+  spec.non_flex_cond B (σ.val ⊔ {new_non_flex_constraint hγ hδ hγδ t hπ})⁻¹ :=
 sorry
 
-lemma non_flexible_union_support_closed_forward :
-  (σ.val ⊔ {new_non_flexible_constraint hγ hδ hγδ t hπ}).domain.support_closed B :=
+lemma non_flex_union_support_closed_forward :
+  (σ.val ⊔ {new_non_flex_constraint hγ hδ hγδ t hπ}).domain.support_closed B :=
 begin
   unfold unary_spec.support_closed,
   simp,
@@ -223,44 +223,44 @@ begin
   sorry,
 end
 
-lemma non_flexible_union_support_closed_backward :
-  (σ.val ⊔ {new_non_flexible_constraint hγ hδ hγδ t hπ}).range.support_closed B :=
+lemma non_flex_union_support_closed_backward :
+  (σ.val ⊔ {new_non_flex_constraint hγ hδ hγδ t hπ}).range.support_closed B :=
 sorry
 
-lemma non_flexible_union_flexible_cond :
-  ∀ C, spec.flexible_cond B (σ.val ⊔ {new_non_flexible_constraint hγ hδ hγδ t hπ}) C :=
+lemma non_flex_union_flex_cond :
+  ∀ C, spec.flex_cond B (σ.val ⊔ {new_non_flex_constraint hγ hδ hγδ t hπ}) C :=
 sorry
 
-lemma non_flexible_union_allowable :
-  spec.allowable B (σ.val ⊔ {new_non_flexible_constraint hγ hδ hγδ t hπ}) :=
+lemma non_flex_union_allowable :
+  spec.allowable B (σ.val ⊔ {new_non_flex_constraint hγ hδ hγδ t hπ}) :=
 { forward :=
-  { one_to_one := non_flexible_union_one_to_one_forward hγ hδ hγδ t hπ,
-    atom_cond := non_flexible_union_atom_cond_forward hγ hδ hγδ t hπ,
-    near_litter_cond := non_flexible_union_near_litter_cond_forward hγ hδ hγδ t hπ,
-    non_flexible_cond := non_flexible_union_non_flexible_cond_forward hγ hδ hγδ t hπ,
-    support_closed := non_flexible_union_support_closed_forward hγ hδ hγδ t hπ },
+  { one_to_one := non_flex_union_one_to_one_forward hγ hδ hγδ t hπ,
+    atom_cond := non_flex_union_atom_cond_forward hγ hδ hγδ t hπ,
+    near_litter_cond := non_flex_union_near_litter_cond_forward hγ hδ hγδ t hπ,
+    non_flex_cond := non_flex_union_non_flex_cond_forward hγ hδ hγδ t hπ,
+    support_closed := non_flex_union_support_closed_forward hγ hδ hγδ t hπ },
   backward :=
-  { one_to_one := non_flexible_union_one_to_one_backward hγ hδ hγδ t hπ,
-    atom_cond := non_flexible_union_atom_cond_backward hγ hδ hγδ t hπ,
-    near_litter_cond := non_flexible_union_near_litter_cond_backward hγ hδ hγδ t hπ,
-    non_flexible_cond := non_flexible_union_non_flexible_cond_backward hγ hδ hγδ t hπ,
+  { one_to_one := non_flex_union_one_to_one_backward hγ hδ hγδ t hπ,
+    atom_cond := non_flex_union_atom_cond_backward hγ hδ hγδ t hπ,
+    near_litter_cond := non_flex_union_near_litter_cond_backward hγ hδ hγδ t hπ,
+    non_flex_cond := non_flex_union_non_flex_cond_backward hγ hδ hγδ t hπ,
     support_closed := by { rw spec.domain_inv,
-      exact non_flexible_union_support_closed_backward hγ hδ hγδ t hπ } },
-  flexible_cond := non_flexible_union_flexible_cond hγ hδ hγδ t hπ }
+      exact non_flex_union_support_closed_backward hγ hδ hγδ t hπ } },
+  flex_cond := non_flex_union_flex_cond hγ hδ hγδ t hπ }
 
-lemma le_non_flexible_union : σ ≤ ⟨_, non_flexible_union_allowable hγ hδ hγδ t hπ⟩ :=
+lemma le_non_flex_union : σ ≤ ⟨_, non_flex_union_allowable hγ hδ hγδ t hπ⟩ :=
 { le := le_sup_left,
   all_flex_domain := begin
     rintro L N' C' hN' hσ₁ (hσ₂ | hσ₂),
     { cases hσ₁ hσ₂ },
-    { simp only [new_non_flexible_constraint, set_like.mem_coe, spec.mem_singleton,
+    { simp only [new_non_flex_constraint, set_like.mem_coe, spec.mem_singleton,
         prod.mk.inj_iff] at hσ₂,
       cases hN' hγ hδ hγδ C hσ₂.2 t (litter.to_near_litter_injective hσ₂.left.left), }
   end,
   all_flex_range := begin
     rintro L N' C' hN' hσ₁ (hσ₂ | hσ₂),
     { cases hσ₁ hσ₂ },
-    { simp only [new_non_flexible_constraint, set_like.mem_coe, spec.mem_singleton,
+    { simp only [new_non_flex_constraint, set_like.mem_coe, spec.mem_singleton,
         prod.mk.inj_iff] at hσ₂,
       exfalso,
       refine hN' hγ hδ hγδ C hσ₂.2 t _,
@@ -271,17 +271,17 @@ lemma le_non_flexible_union : σ ≤ ⟨_, non_flexible_union_allowable hγ hδ 
   all_atoms_domain := begin
     rintro a b L ha C hσ₁ (hσ₂ | hσ₂),
     { cases hσ₁ hσ₂ },
-    { simpa only [new_non_flexible_constraint, set_like.mem_coe, spec.mem_singleton,
+    { simpa only [new_non_flex_constraint, set_like.mem_coe, spec.mem_singleton,
         prod.mk.inj_iff, false_and] using hσ₂ }
   end,
   all_atoms_range := begin
     rintro a b L ha C hσ₁ (hσ₂ | hσ₂),
     { cases hσ₁ hσ₂ },
-    { simpa only [new_non_flexible_constraint, set_like.mem_coe, spec.mem_singleton,
+    { simpa only [new_non_flex_constraint, set_like.mem_coe, spec.mem_singleton,
         prod.mk.inj_iff, false_and] using hσ₂ }
   end }
 
-lemma exists_ge_non_flexible (hγ : γ < β) (hδ : δ < β) (hγδ : γ ≠ δ) {C : path (B : type_index) β}
+lemma exists_ge_non_flex (hγ : γ < β) (hδ : δ < β) (hγδ : γ ≠ δ) {C : path (B : type_index) β}
   (t : tangle_path ((lt_index.mk' hγ (B.path.comp C)) : le_index α))
   (hσ : ∀ c, c ≺ (inr (f_map_path hγ hδ t).to_near_litter,
     (C.cons $ coe_lt_coe.mpr hδ).cons (bot_lt_coe _)) →
@@ -300,10 +300,10 @@ begin
     ⟨σ.val.lower (C.cons $ coe_lt_coe.mpr hδ), this⟩,
   have := struct_perm.derivative (path.nil.cons $ bot_lt_coe _) π.to_struct_perm
      • (f_map_path hγ hδ t).to_near_litter,
-  refine ⟨_, le_non_flexible_union hγ hδ hγδ t hπ, _⟩,
+  refine ⟨_, le_non_flex_union hγ hδ hγδ t hπ, _⟩,
   rw spec.domain_sup,
   right, simpa only [spec.domain, image_singleton, mem_singleton_iff],
 end
 
-end allowable_partial_perm
+end allowable_spec
 end con_nf
